\begin{to_def} 
    \textit{Внешнее умножение} $\Omega^k(U) \times \Omega^l (U) \mapsto \Omega^{k+l} (U)$, можно определить как 
    \begin{equation*}
      \alpha \wedge \beta =
      \frac{(k+l)!}{k!l!} 
       \text{Alt}\, (\alpha \otimes \beta)
       \left[\overset{\mathrm{or}}{=}
                     \text{Alt}\, (\alpha \otimes \beta)\right]
       ,
      \hspace{0.5cm} \text{где} \hspace{0.5cm} 
        \text{Alt}\, (T(\ldots)) = \frac{1}{(k+l)!} \sum_{\sigma \in \Sigma_{k+l}} \sign \sigma \cdot T(\sigma(\ldots)),
    \end{equation*}
    при чём $(dx_1 \wedge \ldots \wedge dx_k)(\partial_1, \ldots, \partial_k) = 1$.
\end{to_def}


Просто так








